first step towards later credits support
This uses le_upd in our definitions of fupd and fupd2, which requires large
changes to our adequacy proofs since the "plainly" laws no longer hold. That
means later credits can be eliminated. What is still missing is a mechanism that
actually generates credits.

src/base_logic/lib/fancy_updates.v
@@ -1,11 +1,11 @@
 From stdpp Require Export coPset.
 From iris.algebra Require Import gmap auth agree gset coPset.
 From iris.proofmode Require Import tactics.
-From Perennial.base_logic.lib Require Export own.
+From Perennial.base_logic.lib Require Export own later_credits.
 From Perennial.base_logic.lib Require Import wsat.
 From iris.prelude Require Import options.
 Export invGS.
-Import uPred.
+Import uPred le_upd.
 
 (** * Suffix subsets *)
 Fixpoint coPset_suffixes_of_raw (p : positive) (E: coPset_raw) : coPset_raw :=
@@ -59,7 +59,7 @@ Local Hint Extern 0 (AlwaysEn ## MaybeEn1 _) => apply coPset_inl_inr_disj : core
 Local Hint Extern 0 (AlwaysEn ## MaybeEn2 _) => apply coPset_inl_inr_disj : core.
 
 Definition uPred_fupd_def `{!invGS Σ} (E1 E2 : coPset) (P : iProp Σ) : iProp Σ :=
-  wsat_all ∗ ownE (AlwaysEn ∪ MaybeEn1 E1) ==∗ ◇ (wsat_all ∗ ownE (AlwaysEn ∪ MaybeEn1 E2) ∗ P).
+  wsat_all ∗ ownE (AlwaysEn ∪ MaybeEn1 E1) -∗ |==£> ◇ (wsat_all ∗ ownE (AlwaysEn ∪ MaybeEn1 E2) ∗ P).
 Definition uPred_fupd_aux : seal (@uPred_fupd_def). Proof. by eexists. Qed.
 Definition uPred_fupd := uPred_fupd_aux.(unseal).
 Global Arguments uPred_fupd {Σ _}.
@@ -142,27 +142,6 @@ Global Instance uPred_bi_fupd `{!invGS Σ} : BiFUpd (uPredI (iResUR Σ)) :=
 Global Instance uPred_bi_bupd_fupd `{!invGS Σ} : BiBUpdFUpd (uPredI (iResUR Σ)).
 Proof. rewrite /BiBUpdFUpd uPred_fupd_eq. by iIntros (E P) ">? [$ $] !> !>". Qed.
 
-Lemma uPred_bi_fupd_plainly `{!invGS Σ} : BiFUpdPlainly (uPredI (iResUR Σ)).
-Proof.
-  split.
-  - rewrite uPred_fupd_eq /uPred_fupd_def. iIntros (E P) "H [Hw HE]".
-    iAssert (◇ ■ P)%I as "#>HP".
-    { by iMod ("H" with "[$]") as "(_ & _ & HP)". }
-    by iFrame.
-  - rewrite uPred_fupd_eq /uPred_fupd_def. iIntros (E P Q) "[H HQ] [Hw HE]".
-    iAssert (◇ ■ P)%I as "#>HP".
-    { by iMod ("H" with "HQ [$]") as "(_ & _ & HP)". }
-    by iFrame.
-  - rewrite uPred_fupd_eq /uPred_fupd_def. iIntros (E P) "H [Hw HE]".
-    iAssert (▷ ◇ ■ P)%I as "#HP".
-    { iNext. by iMod ("H" with "[$]") as "(_ & _ & HP)". }
-    iFrame. iIntros "!> !> !>". by iMod "HP".
-  - rewrite uPred_fupd_eq /uPred_fupd_def. iIntros (E A Φ) "HΦ [Hw HE]".
-    iAssert (◇ ■ ∀ x : A, Φ x)%I as "#>HP".
-    { iIntros (x). by iMod ("HΦ" with "[$Hw $HE]") as "(_&_&?)". }
-    by iFrame.
-Qed.
-
 Lemma ownE_mono_le_acc `{!invGS Σ} E1 E2:
   E1 ⊆ E2 →
   ownE E2 -∗ ownE E1 ∗ (ownE E1 -∗ ownE E2).
@@ -177,37 +156,67 @@ Proof.
   iIntros (?) "H". by iDestruct (ownE_mono_le_acc with "H") as "($&_)".
 Qed.
 
-Local Lemma fupd_plain_soundness `{!invGpreS Σ} E1 E2 (P: iProp Σ) `{!Plain P} :
-  (∀ `{Hinv: !invGS Σ}, ⊢ |={E1,E2}=> P) → ⊢ P.
+(** [lc_fupd_elim_later] allows to eliminate a later from a hypothesis at an update.
+  This is typically used as [iMod (lc_fupd_elim_later with "Hcredit HP") as "HP".],
+  where ["Hcredit"] is a credit available in the context and ["HP"] is the
+  assumption from which a later should be stripped. *)
+Lemma lc_fupd_elim_later `{!invGS Σ} E P :
+   £1 -∗ (▷ P) -∗ |={E}=> P.
 Proof.
-  iIntros (Hfupd). apply later_soundness. iMod wsat_alloc as (Hinv) "[Hw HE]".
-  iAssert (|={⊤,E2}=> P)%I as "H".
-  { iMod (fupd_mask_subseteq E1) as "_"; first done. iApply Hfupd. }
+  iIntros "Hf Hupd".
   rewrite uPred_fupd_eq /uPred_fupd_def.
-  iMod ("H" with "[$Hw HE]") as "[Hw [HE >H']]"; iFrame.
-  iApply (ownE_weaken with "HE"). set_solver.
+  iIntros "[$ $]". iApply (le_upd_later with "Hf").
+  iNext. by iModIntro.
 Qed.
 
-Lemma step_fupdN_soundness `{!invGpreS Σ} φ n :
+(** If the goal is a fancy update, this lemma can be used to make a later appear
+  in front of it in exchange for a later credit.
+  This is typically used as [iApply (lc_fupd_add_later with "Hcredit")],
+  where ["Hcredit"] is a credit available in the context. *)
+Lemma lc_fupd_add_later `{!invGS Σ} E1 E2 P :
+  £1 -∗ (▷ |={E1, E2}=> P) -∗ |={E1, E2}=> P.
+Proof.
+  iIntros "Hf Hupd". iApply (fupd_trans E1 E1).
+  iApply (lc_fupd_elim_later with "Hf Hupd").
+Qed.
+
+Local Existing Instance inv_lcPreG.
+
+Lemma fupd_soundness `{!invGpreS Σ} n E1 E2 (φ : Prop) :
+  (∀ `{Hinv: !invGS Σ}, £ n ⊢@{iPropI Σ} |={E1,E2}=> ⌜φ⌝) → φ.
+Proof.
+  iIntros (Hfupd).
+  eapply (lc_soundness (Σ:=Σ) (S n)). intros Hc. rewrite lc_succ.
+  iIntros "[Hone Hn]". rewrite -le_upd_trans. iApply bupd_le_upd.
+  iMod wsat_alloc as (Hinv ->) "[Hw HE]".
+  iAssert (|={⊤,E2}=> ⌜φ⌝)%I with "[Hn]" as "H".
+  { iMod (fupd_mask_subseteq E1) as "_"; first done. by iApply (Hfupd _). }
+  rewrite uPred_fupd_eq /uPred_fupd_def.
+  iModIntro. iMod ("H" with "[$Hw HE]") as "[Hw [HE H']]".
+  { iApply (ownE_weaken with "HE"). set_solver. }
+  iPoseProof (except_0_into_later with "H'") as "H'".
+  iApply (le_upd_later with "Hone"). iNext. done.
+Qed.
+
+Lemma step_fupdN_soundness `{!invGpreS Σ} n φ :
   (∀ `{Hinv: !invGS Σ}, ⊢@{iPropI Σ} |={⊤,∅}=> |={∅}▷=>^n ⌜ φ ⌝) →
   φ.
 Proof.
-  pose local_instance := uPred_bi_fupd_plainly.
   intros Hiter.
-  apply (soundness (M:=iResUR Σ) _  (S n)); simpl.
-  apply (fupd_plain_soundness ⊤ ⊤ _)=> Hinv.
-  iPoseProof (Hiter Hinv) as "H". clear Hiter.
-  iApply fupd_plainly_mask_empty. iMod "H".
-  iMod (step_fupdN_plain with "H") as "H". iModIntro.
-  rewrite -later_plainly -laterN_plainly -later_laterN laterN_later.
-  iNext. iMod "H" as %Hφ. auto.
+  eapply (fupd_soundness n)=> Hinv. iIntros "Hn".
+  iMod Hiter as "Hupd". clear Hiter.
+  iInduction n as [|n] "IH"; simpl.
+  - by iModIntro.
+  - rewrite lc_succ. iDestruct "Hn" as "[Hone Hn]".
+    iMod "Hupd". iMod (lc_fupd_elim_later with "Hone Hupd") as "> Hupd".
+    by iApply ("IH" with "Hn Hupd").
 Qed.
 
-Lemma step_fupdN_soundness' `{!invGpreS Σ} φ n :
+Lemma step_fupdN_soundness' `{!invGpreS Σ} n φ :
   (∀ `{Hinv: !invGS Σ}, ⊢@{iPropI Σ} |={⊤}[∅]▷=>^n ⌜ φ ⌝) →
   φ.
 Proof.
-  iIntros (Hiter). eapply (step_fupdN_soundness _ n)=>Hinv. destruct n as [|n].
+  iIntros (Hiter). eapply (step_fupdN_soundness n)=>Hinv. destruct n as [|n].
   { by iApply fupd_mask_intro_discard; [|iApply (Hiter Hinv)]. }
    simpl in Hiter |- *. iMod Hiter as "H". iIntros "!>!>!>".
   iMod "H". clear. iInduction n as [|n] "IH"; [by iApply fupd_mask_intro_discard|].
